src/Std/Data/HashSet/RawLemmas.lean
@@ -854,18 +854,34 @@ theorem isEmpty_filter_iff [EquivBEq α] [LawfulHashable α]
     {f : α → Bool} (h : m.WF) :
     (m.filter f).isEmpty ↔
       ∀ (k : α) (h : k ∈ m), f (m.get k h) = false :=
-  HashMap.Raw.isEmpty_filter_key_iff h.out
+  HashMap.Raw.isEmpty_filter_iff h.out
 
 theorem isEmpty_filter_eq_false_iff [EquivBEq α] [LawfulHashable α]
     {f : α → Bool} (h : m.WF) :
     (m.filter f).isEmpty = false ↔
       ∃ (k : α) (h : k ∈ m), f (m.get k h) :=
-  HashMap.Raw.isEmpty_filter_key_eq_false_iff h.out
+  HashMap.Raw.isEmpty_filter_eq_false_iff h.out
+
+@[simp]
+theorem mem_filter [EquivBEq α] [LawfulHashable α]
+    {f : α → Bool} {k : α} (h : m.WF) :
+    (k ∈ m.filter f) ↔ ∃ (h' : k ∈ m), f (m.get k h') :=
+  HashMap.Raw.mem_filter h.out
+
+theorem mem_of_mem_filter [EquivBEq α] [LawfulHashable α]
+    {f : α → Bool} {k : α} (h : m.WF) :
+    k ∈ (m.filter f) → k ∈ m :=
+  HashMap.Raw.mem_of_mem_filter h.out
 
 theorem size_filter_le_size [EquivBEq α] [LawfulHashable α]
     {f : α → Bool} (h : m.WF) :
     (m.filter f).size ≤ m.size :=
   HashMap.Raw.size_filter_le_size h.out
+
+theorem size_filter_eq_size_iff [EquivBEq α] [LawfulHashable α]
+    {f : α → Bool} (h : m.WF) :
+    (m.filter f).size = m.size ↔ ∀ (k : α) (h : k ∈ m), f (m.get k h) :=
+  HashMap.Raw.size_filter_eq_size_iff h.out
 
 theorem filter_equiv_self_iff [EquivBEq α] [LawfulHashable α]
     {f : (a : α) → Bool} (h : m.WF) :
@@ -873,53 +889,27 @@ theorem filter_equiv_self_iff [EquivBEq α] [LawfulHashable α]
   ⟨fun h' => (HashMap.Raw.filter_equiv_self_iff h.out).mp h'.1,
     fun h' => ⟨(HashMap.Raw.filter_equiv_self_iff h.out).mpr h'⟩⟩
 
-theorem size_filter_eq_size_iff [EquivBEq α] [LawfulHashable α]
-    {f : α → Bool} (h : m.WF) :
-    (m.filter f).size = m.size ↔ ∀ (k : α) (h : k ∈ m), f (m.get k h) :=
-  HashMap.Raw.size_filter_key_eq_size_iff h.out
-
-theorem mem_of_mem_filter [EquivBEq α] [LawfulHashable α]
-    {f : α → Bool} {k : α} (h : m.WF) :
-    k ∈ (m.filter f) → k ∈ m :=
-  HashMap.Raw.mem_of_mem_filter h.out
-
-theorem mem_filter [EquivBEq α] [LawfulHashable α]
-    {f : α → Bool} {k : α} (h : m.WF) :
-    (k ∈ m.filter f) ↔ ∃ (h' : k ∈ m),
-      f (m.get k h') :=
-  HashMap.Raw.mem_filter h.out
-
+@[simp]
 theorem get?_filter [EquivBEq α] [LawfulHashable α]
     {f : α → Bool} {k : α} (h : m.WF) :
-    (m.filter f).get? k =
-    (m.get? k).filter f := by
-  have := HashMap.Raw.getKey?_filter h.out (k:=k) (f:= fun k _ => f k)
-  simp only [Option.pfilter_eq_filter] at this
-  exact this
+    (m.filter f).get? k = (m.get? k).filter f :=
+  HashMap.Raw.getKey?_filter_key h.out
 
+@[simp]
 theorem get_filter [EquivBEq α] [LawfulHashable α]
     {f : α → Bool} {k : α} {h'} (h : m.WF) :
-    (m.filter f).get k h' =
-    (m.get k (mem_of_mem_filter h h')) := by
-  have := HashMap.Raw.getKey_filter h.out (k:=k) (f:= fun k _ => f k) (h':= h')
-  simp only [Option.pfilter_eq_filter] at this
-  exact this
+    (m.filter f).get k h' = (m.get k (mem_of_mem_filter h h')) :=
+  HashMap.Raw.getKey_filter h.out
 
-theorem get!_filter_key [EquivBEq α] [LawfulHashable α] [Inhabited α]
+theorem get!_filter [EquivBEq α] [LawfulHashable α] [Inhabited α]
     {f : α → Bool} {k : α} (h : m.WF) :
-    (m.filter f).get! k =
-    ((m.get? k).filter f).get! := by
-  have := HashMap.Raw.getKey!_filter h.out (k:=k) (f:= fun k _ => f k)
-  simp only [Option.pfilter_eq_filter] at this
-  exact this
+    (m.filter f).get! k = ((m.get? k).filter f).get! :=
+  HashMap.Raw.getKey!_filter_key h.out
 
 theorem getD_filter [EquivBEq α] [LawfulHashable α]
     {f : α → Bool} {k fallback : α} (h : m.WF) :
-    (m.filter f).getD k fallback =
-    ((m.get? k).filter f).getD fallback := by
-  have := HashMap.Raw.getKeyD_filter h.out (k:=k) (f:= fun k _ => f k) (fallback := fallback)
-  simp only [Option.pfilter_eq_filter] at this
-  exact this
+    (m.filter f).getD k fallback = ((m.get? k).filter f).getD fallback :=
+  HashMap.Raw.getKeyD_filter_key h.out
 
 end filter
 
